Finalmente,
\begin{equation}
\Lambda = \left\{ \frac{\hat{\sigma}^2_c}{\hat{\sigma}^2} \right\}^{\frac{n+m}{2}} 
= \left\{ \frac{\frac{\sum_{i=1}^n (x_i - \bar{x})^2 + \sum_{i=1}^m (y_i - \bar{y})^2}{n+m}}{\frac{\sum_{i=1}^n (x_i - \hat{\mu})^2 + \sum_{i=1}^m (y_i - \hat{\mu})^2}{n+m}} \right\}^{\frac{n+m}{2}}.
\end{equation}

Note que
\begin{equation}
\sum_{i=1}^n (x_i - \hat{\mu}_x)^2 + \sum_{i=1}^m (y_i - \hat{\mu}_y)^2 
= \sum_{i=1}^n (x_i - \bar{x})^2 + n(\bar{x} - \hat{\mu})^2 
+ \sum_{i=1}^m (y_i - \bar{y})^2 + m(\bar{y} - \hat{\mu})^2
\end{equation}
\[
\underbrace{(n-1) s_x^2}_{\text{variância amostral de $x$}} \quad\quad \underbrace{(m-1) s_y^2}_{\text{variância amostral de $y$}}
\]

E, para
\begin{equation}
R(\bar{x}, \bar{y}) = \frac{n(\bar{x} - \hat{\mu})^2 + m(\bar{y} - \hat{\mu})^2}{(n-1) s_x^2 + (m-1) s_y^2},
\end{equation}
temos
\begin{equation}
\Lambda = \left\{ \frac{1}{1 + R(\bar{x}, \bar{y})} \right\}^{\frac{n+m}{2}} 
= \left\{ 1 + R(\bar{x}, \bar{y}) \right\}^{-\frac{n+m}{2}}.
\end{equation}

Ainda,
\begin{equation}
n(\bar{x} - \hat{\mu})^2 + m(\bar{y} - \hat{\mu})^2 
= n\left[ \bar{x} - \frac{n\bar{x} + m\bar{y}}{n+m} \right]^2 
+ m\left[ \bar{y} - \frac{n\bar{x} + m\bar{y}}{n+m} \right]^2
\end{equation}
\begin{equation}
= n\left[ \frac{m\bar{x} - m\bar{y}}{n+m} \right]^2 
+ m\left[ \frac{n\bar{y} - n\bar{x}}{n+m} \right]^2
\end{equation}
\begin{equation}
= \frac{nm^2}{(n+m)^2} (\bar{x} - \bar{y})^2 + \frac{mn^2}{(n+m)^2} (\bar{x} - \bar{y})^2 
= \frac{nm}{n+m} (\bar{x} - \bar{y})^2.
\end{equation}

