Usualmente, os estimadores invariantes de MV para $\mu_x$, $\mu_y$, $\sigma_x^2$, $\sigma_y^2$ são dados por:
\begin{equation}
\hat{\mu}_x = \bar{X}, \quad \hat{\mu}_y = \bar{Y}, \quad \hat{\sigma}_x^2 = \frac{1}{n} \sum_{i=1}^n (X_i - \bar{X})^2, \quad \hat{\sigma}_y^2 = \frac{1}{m} \sum_{i=1}^m (Y_i - \bar{Y})^2
\end{equation}
respectivamente. Aqui,
\begin{equation}
\Theta_0 = \{ (\mu_x, \mu_y, \sigma_x, \sigma_y) : \mu_x, \mu_y \in \mathbb{R} \ \text{e} \ \sigma_x = \sigma_y \in \mathbb{R}_+ \}
\end{equation}
\begin{equation}
\Theta = \{ (\mu_x, \mu_y, \sigma_x, \sigma_y) : \mu_x, \mu_y \in \mathbb{R} \ \text{e} \ \sigma_x^2, \sigma_y^2 \in \mathbb{R}_+ \}
\end{equation}

Dado,
\begin{equation}
\sup_{\Theta_0} \{ L(\Theta) \} = (2\pi)^{-\frac{n+m}{2}} (\tilde{\sigma}^2)^{-\frac{n+m}{2}} \cdot \exp\left\{ -\frac{1}{2\tilde{\sigma}^2} \left[ (n-1) s_x^2 + (m-1) s_y^2 \right] \right\}
\end{equation}
em que $s_x^2$ é uma observação de $S_x^2$ e $s_y^2$ é uma observação de $S_y^2$. Logo,
\begin{equation}
\sup_{\Theta_0} \{ L(\Theta) \} = (2\pi \tilde{\sigma}^2)^{-\frac{n+m}{2}} e^{-\frac{n+m}{2}}
\end{equation}

\begin{equation}
\sup_{\Theta} \{ L(\Theta) \} = (2\pi)^{-\frac{n+m}{2}} \left( \hat{\sigma}_x^n \hat{\sigma}_y^m \right)^{-\frac{1}{2}} e^{-\frac{n+m}{2}}
\end{equation}

Dado, temos que
\begin{equation}
\Lambda = \frac{(\hat{\sigma}_x^2)^{\frac{n}{2}} (\hat{\sigma}_y^2)^{\frac{m}{2}}}{(\tilde{\sigma}^2)^{\frac{n+m}{2}}} = \frac{(\hat{\sigma}_x^2)^{\frac{n}{2}} (\hat{\sigma}_y^2)^{\frac{m}{2}}}{\left[ (mn)^{-1} (n \hat{\sigma}_x^2 + m \hat{\sigma}_y^2) \right]^{\frac{n+m}{2}}}
\end{equation}

