\begin{equation}
p = \frac{1}{2}: \quad \frac{1}{2} e^{-t\frac{\sqrt{n}}{n}} \left[ 1 + e^{\frac{2t}{\sqrt{n}}} \right]
\end{equation}

\begin{equation}
= \frac{1}{2^n} \left[ e^{-t\sqrt{n}} + e^{t\sqrt{n}} \right]
\end{equation}

\begin{equation}
M_{Un}(t) = \frac{1}{2} \left( e^{-t\frac{\sqrt{n}}{n}} + e^{t\frac{\sqrt{n}}{n}} \right)^n
\end{equation}

\begin{equation}
= \frac{1}{2} \left[ \left( 1 - \frac{t}{\sqrt{n}} + \frac{t^2}{2n} + o\left( \frac{t^2}{n} \right) \right) \left( 1 + \frac{t}{\sqrt{n}} + \frac{t^2}{2n} + o\left( \frac{t^2}{n} \right) \right) \right]^n
\end{equation}

\begin{equation}
= \frac{1}{2} \left[ 2 + \frac{t^2}{n} + o\left( \frac{t^2}{n} \right) \right]^n
\end{equation}

\begin{equation}
R_n = o\left( \max\left[ \frac{t^2}{n}, \frac{t^2}{n^2} \right] \right)
\end{equation}

\begin{equation}
= \left\{ \frac{1}{2} + \frac{t^2}{n} + R_n \right\}
\end{equation}

Em que $R_n = O(n^{-2})$. Assim, de

\begin{equation}
\lim_{n \to \infty} \left( 1 + \frac{t^2}{2n} \right)^n = e^{t^2/2}
\end{equation}

\begin{equation}
M_{Un}(t) \xrightarrow[n \to \infty]{} e^{t^2/2} = M_U(t)
\end{equation}

que Ã© a fgm de $Z \sim N(0,1)$, logo

\begin{equation}
U_n \xrightarrow[n \to \infty]{} Z
\end{equation}